Continue

src/Set_Semantics.thy
@@ -5,7 +5,7 @@ begin
 section \<open>Syntax and Semantics\<close>
 
 datatype (vars_term: 'a) pset_term = 
-  Empty (\<open>\<emptyset>\<close>) | is_Var: Var 'a |
+  Empty nat (\<open>\<emptyset> _\<close>) | is_Var: Var 'a |
   Union "'a pset_term" "'a pset_term" (infixr \<open>\<squnion>\<^sub>s\<close> 60) |
   Inter "'a pset_term" "'a pset_term" (infixr \<open>\<sqinter>\<^sub>s\<close> 70) |
   Diff "'a pset_term" "'a pset_term"  (infixl \<open>-\<^sub>s\<close> 80) |
@@ -22,7 +22,7 @@ type_synonym 'a pset_fm = "'a pset_atom fm"
 type_synonym 'a branch = "'a pset_fm list"
 
 fun I\<^sub>s\<^sub>t :: "('a \<Rightarrow> V) \<Rightarrow> 'a pset_term \<Rightarrow> V" where
-  "I\<^sub>s\<^sub>t v \<emptyset> = 0"
+  "I\<^sub>s\<^sub>t v (\<emptyset> n) = 0"
 | "I\<^sub>s\<^sub>t v (Var x) = v x"
 | "I\<^sub>s\<^sub>t v (s1 \<squnion>\<^sub>s s2) = I\<^sub>s\<^sub>t v s1 \<squnion> I\<^sub>s\<^sub>t v s2"
 | "I\<^sub>s\<^sub>t v (s1 \<sqinter>\<^sub>s s2) = I\<^sub>s\<^sub>t v s1 \<sqinter> I\<^sub>s\<^sub>t v s2"
@@ -124,7 +124,7 @@ lemma subfmsD:
 subsection \<open>Subterms\<close>
 
 fun subterms_term :: "'a pset_term \<Rightarrow> 'a pset_term set"  where
-  "subterms_term \<emptyset> = {\<emptyset>}"
+  "subterms_term (\<emptyset> n) = {\<emptyset> n}"
 | "subterms_term (Var i) = {Var i}"
 | "subterms_term (t1 \<squnion>\<^sub>s t2) = {t1 \<squnion>\<^sub>s t2} \<union> subterms_term t1 \<union> subterms_term t2"
 | "subterms_term (t1 \<sqinter>\<^sub>s t2) = {t1 \<sqinter>\<^sub>s t2} \<union> subterms_term t1 \<union> subterms_term t2"
@@ -375,70 +375,5 @@ lemma subterms_atom_nonempty[simp]: "subterms_atom l \<noteq> {}"
 
 lemma subterms_fm_nonempty[simp]: "subterms_fm \<phi> \<noteq> {}"
   by (induction \<phi>) auto
-
-section \<open>Typing\<close>
-
-datatype 'a lvl = GT 'a | EQ 'a
-
-fun eq_lvl :: "nat lvl \<Rightarrow> nat lvl \<Rightarrow> nat lvl option" where
-  "eq_lvl (GT l) (GT k) = Some (GT (max l k))"
-| "eq_lvl (GT l) (EQ k) = (if k > l then Some (EQ k) else None)"
-| "eq_lvl (EQ k) (GT l) = (if k > l then Some (EQ k) else None)"
-| "eq_lvl (EQ l) (EQ k) = (if l = k then Some (EQ k) else None)"
-
-fun suc_lvl :: "nat lvl \<Rightarrow> nat lvl \<Rightarrow> bool" where
-  "suc_lvl (GT l) (GT k) \<longleftrightarrow> True"
-| "suc_lvl (GT l) (EQ k) \<longleftrightarrow> k = Suc (Suc l)"
-| "suc_lvl (EQ l) (GT k) \<longleftrightarrow> l \<ge> k"
-| "suc_lvl (EQ l) (EQ k) \<longleftrightarrow> Suc l = k"
-
-fun type_term :: "('a \<Rightarrow> nat) \<Rightarrow> 'a pset_term \<Rightarrow> nat lvl option" where
-    "type_term _ \<emptyset> = Some (GT 0)"
-  | "type_term v (Var x) = Some (EQ (v x))"
-  | "type_term v (Single t) = map_option (map_lvl Suc) (type_term v t)"
-  | "type_term v (s \<squnion>\<^sub>s t) = do {
-                              ts <- type_term v s;
-                              tt <- type_term v t;
-                              lvl <- eq_lvl ts tt;
-                              if lvl \<noteq> EQ 0 then Some lvl else None
-                            }"
-  | "type_term v (s \<sqinter>\<^sub>s t) = do {
-                              ts <- type_term v s;
-                              tt <- type_term v t;
-                              lvl <- eq_lvl ts tt;
-                              if lvl \<noteq> EQ 0 then Some lvl else None
-                            }"
-  | "type_term v (s -\<^sub>s t) = do {
-                              ts <- type_term v s;
-                              tt <- type_term v t;
-                              lvl <- eq_lvl ts tt;
-                              if lvl \<noteq> EQ 0 then Some lvl else None
-                            }"
-
-consts types :: "('a \<Rightarrow> nat) \<Rightarrow> 'b \<Rightarrow> bool" ("_ \<turnstile> _" 45)
-
-inductive types_pset_atom :: "('a \<Rightarrow> nat) \<Rightarrow> 'a pset_atom \<Rightarrow> bool" where
-  "\<lbrakk> type_term v s = Some l; type_term v t = Some k; eq_lvl l k = Some n \<rbrakk>
-  \<Longrightarrow> types_pset_atom v (s =\<^sub>s t)"
-| "\<lbrakk> type_term v s = Some l; type_term v t = Some k; suc_lvl l k\<rbrakk> \<Longrightarrow> types_pset_atom v (s \<in>\<^sub>s t)"
-
-adhoc_overloading types types_pset_atom
-
-definition types_pset_fm :: "('a \<Rightarrow> nat) \<Rightarrow> 'a pset_fm \<Rightarrow> bool" where
-  "types_pset_fm v \<phi> \<equiv> (\<forall>a \<in> atoms \<phi>. v \<turnstile> a)"
-
-adhoc_overloading types types_pset_fm
-
-definition urelem :: "'a pset_fm \<Rightarrow> 'a pset_term \<Rightarrow> bool" where
-  "urelem \<phi> t \<equiv> (\<exists>v. v \<turnstile> \<phi> \<and> t \<in> subterms \<phi> \<and> type_term v t = Some (EQ 0))"
-
-lemma map_lvl_Suc_neq_EQ_0[simp]: "map_lvl Suc z \<noteq> EQ 0"
-  by (cases z) auto
-
-lemma is_Var_if_type_term_0: "type_term v t = Some (EQ 0) \<Longrightarrow> is_Var t"
-  by (induction t) (auto split: if_splits Option.bind_splits)
-
-lemma is_Var_if_urelem: "urelem \<phi> t \<Longrightarrow> is_Var t"
-  unfolding urelem_def using is_Var_if_type_term_0 by blast
 
 end
