src/Typing.thy
@@ -1,0 +1,328 @@
+theory Typing
+  imports Set_Calculus
+begin
+
+section \<open>Typing\<close>
+
+(*
+datatype 'a lvl = is_GT: GT 'a | EQ 'a
+
+fun eq_lvl :: "nat lvl \<Rightarrow> nat lvl \<Rightarrow> nat lvl option" where
+  "eq_lvl (GT l) (GT k) = Some (GT (max l k))"
+| "eq_lvl (GT l) (EQ k) = (if k > l then Some (EQ k) else None)"
+| "eq_lvl (EQ k) (GT l) = (if k > l then Some (EQ k) else None)"
+| "eq_lvl (EQ l) (EQ k) = (if l = k then Some (EQ k) else None)"
+
+fun suc_lvl :: "nat lvl \<Rightarrow> nat lvl \<Rightarrow> bool" where
+  "suc_lvl (GT l) (GT k) \<longleftrightarrow> True"
+| "suc_lvl (GT l) (EQ k) \<longleftrightarrow> k \<ge> Suc (Suc l)"
+| "suc_lvl (EQ l) (GT k) \<longleftrightarrow> l \<ge> k"
+| "suc_lvl (EQ l) (EQ k) \<longleftrightarrow> Suc l = k"
+*)
+
+fun type_term :: "('a \<Rightarrow> nat) \<Rightarrow> 'a pset_term \<Rightarrow> nat option" where
+    "type_term _ (\<emptyset> n) = Some (Suc n)"
+  | "type_term v (Var x) = Some (v x)"
+  | "type_term v (Single t) = map_option Suc (type_term v t)"
+  | "type_term v (s \<squnion>\<^sub>s t) = do {
+                              ts <- type_term v s;
+                              tt <- type_term v t;
+                              if ts = tt \<and> ts \<noteq> 0 then Some ts else None
+                            }"
+  | "type_term v (s \<sqinter>\<^sub>s t) = do {
+                              ts <- type_term v s;
+                              tt <- type_term v t;
+                              if ts = tt \<and> ts \<noteq> 0 then Some ts else None
+                            }"
+  | "type_term v (s -\<^sub>s t) = do {
+                              ts <- type_term v s;
+                              tt <- type_term v t;
+                              if ts = tt \<and> ts \<noteq> 0 then Some ts else None
+                            }"
+
+declare type_term.simps[simp del]
+
+consts types :: "('a \<Rightarrow> nat) \<Rightarrow> 'b \<Rightarrow> bool" ("_ \<turnstile> _" 45)
+
+inductive types_pset_atom :: "('a \<Rightarrow> nat) \<Rightarrow> 'a pset_atom \<Rightarrow> bool" where
+  "\<lbrakk> type_term v s = Some l; type_term v t = Some l \<rbrakk> \<Longrightarrow> types_pset_atom v (s =\<^sub>s t)"
+| "\<lbrakk> type_term v s = Some l; type_term v t = Some (Suc l)\<rbrakk> \<Longrightarrow> types_pset_atom v (s \<in>\<^sub>s t)"
+
+adhoc_overloading types types_pset_atom
+
+inductive_cases types_pset_atom_Member_cases:
+  "v \<turnstile> s \<in>\<^sub>s t1 \<squnion>\<^sub>s t2" "v \<turnstile> s \<in>\<^sub>s t1 \<sqinter>\<^sub>s t2" "v \<turnstile> s \<in>\<^sub>s t1 -\<^sub>s t2" "v \<turnstile> s \<in>\<^sub>s Single t"
+
+definition types_pset_fm :: "('a \<Rightarrow> nat) \<Rightarrow> 'a pset_fm \<Rightarrow> bool" where
+  "types_pset_fm v \<phi> \<equiv> (\<forall>a \<in> atoms \<phi>. v \<turnstile> a)"
+
+adhoc_overloading types types_pset_fm
+
+definition urelem :: "'a pset_fm \<Rightarrow> 'a pset_term \<Rightarrow> bool" where
+  "urelem \<phi> t \<equiv> (\<exists>v. v \<turnstile> \<phi> \<and> t \<in> subterms \<phi> \<and> type_term v t = Some 0)"
+
+lemma is_Var_if_type_term_0: "type_term v t = Some 0 \<Longrightarrow> is_Var t"
+  by (induction t) (auto simp: type_term.simps split: if_splits Option.bind_splits)
+
+lemma is_Var_if_urelem: "urelem \<phi> t \<Longrightarrow> is_Var t"
+  unfolding urelem_def using is_Var_if_type_term_0 by blast
+
+lemma types_fmD:
+  "v \<turnstile> And p q \<Longrightarrow> v \<turnstile> p"
+  "v \<turnstile> And p q \<Longrightarrow> v \<turnstile> q"
+  "v \<turnstile> Or p q \<Longrightarrow> v \<turnstile> p"
+  "v \<turnstile> Or p q \<Longrightarrow> v \<turnstile> q"
+  "v \<turnstile> Neg p \<Longrightarrow> v \<turnstile> p"
+  "v \<turnstile> Atom a \<Longrightarrow> v \<turnstile> a"
+  unfolding types_pset_fm_def using fm.set_intros by auto
+
+lemma types_fmI:
+  "v \<turnstile> p \<Longrightarrow> v \<turnstile> q \<Longrightarrow> v \<turnstile> And p q"
+  "v \<turnstile> p \<Longrightarrow> v \<turnstile> q \<Longrightarrow> v \<turnstile> Or p q"
+  "v \<turnstile> p \<Longrightarrow> v \<turnstile> Neg p"
+  "v \<turnstile> a \<Longrightarrow> v \<turnstile> Atom a"
+  unfolding types_pset_fm_def using fm.set_intros by auto
+
+
+(*
+lemma type_term_Elem_the_I:
+  assumes "type_term v s = Some ls"
+          "\<not> Option.is_none (type_term v t)" "suc_lvl ls (the (type_term v t))"
+  shows "v \<turnstile> s \<in>\<^sub>s t"
+  using assms types_pset_atom.intros(2)
+  by (metis Option.is_none_def option.exhaust_sel) *)
+
+(*
+lemma type_term_suc_lvl_D:
+  assumes "type_term v s = Some ls" "type_term v (f t1 t2) = Some lt" "f \<in> {(\<squnion>\<^sub>s), (\<sqinter>\<^sub>s), (-\<^sub>s)}"
+  assumes "suc_lvl ls lt"
+  shows "\<not> Option.is_none (type_term v t1) \<and> suc_lvl ls (the (type_term v t1))"
+        "\<not> Option.is_none (type_term v t2) \<and> suc_lvl ls (the (type_term v t2))"
+  using assms
+  by (fastforce simp: type_term.simps dest: suc_lvlD_if_eq_lvl split: if_splits Option.bind_splits)+
+*)
+
+lemma types_pset_atom_Member_D:
+  assumes "v \<turnstile> s \<in>\<^sub>s f t1 t2" "f \<in> {(\<squnion>\<^sub>s), (\<sqinter>\<^sub>s), (-\<^sub>s)}"
+  shows "v \<turnstile> s \<in>\<^sub>s t1" "v \<turnstile> s \<in>\<^sub>s t2"
+proof -
+  from assms obtain ls where
+    "type_term v s = Some ls" "type_term v (f t1 t2) = Some (Suc ls)"
+    using types_pset_atom.simps by fastforce
+  with assms have "v \<turnstile> s \<in>\<^sub>s t1 \<and> v \<turnstile> s \<in>\<^sub>s t2"
+    by (auto simp: type_term.simps types_pset_atom.simps split: if_splits Option.bind_splits)
+  then show "v \<turnstile> s \<in>\<^sub>s t1" "v \<turnstile> s \<in>\<^sub>s t2"
+    by blast+
+qed
+
+lemmas types_pset_atom_Member_Union_D[simplified] = types_pset_atom_Member_D[where ?f="(\<squnion>\<^sub>s)"]
+   and types_pset_atom_Member_Inter_D[simplified] = types_pset_atom_Member_D[where ?f="(\<sqinter>\<^sub>s)"]
+   and types_pset_atom_Member_Diff_D[simplified] = types_pset_atom_Member_D[where ?f="(-\<^sub>s)"]
+
+lemma type_term_eq_if_mem_subterms:
+  fixes \<phi> :: "'a pset_fm"
+  assumes "v \<turnstile> \<phi>"
+  assumes "f t1 t2 \<in> subterms \<phi>" "f \<in> {(\<squnion>\<^sub>s), (\<sqinter>\<^sub>s), (-\<^sub>s)}"
+  shows "\<not> Option.is_none (type_term v t1)"
+        "type_term v t1 = type_term v t2"
+proof -
+  from assms obtain a :: "'a pset_atom" where atom: "v \<turnstile> a" "f t1 t2 \<in> subterms a"
+    unfolding types_pset_fm_def by (induction \<phi>) auto
+  then obtain g s t where "g \<in> {(\<in>\<^sub>s), (=\<^sub>s)}" "a = g s t"
+    by (cases a) auto
+  obtain t' l where "type_term v t' = Some l" "f t1 t2 \<in> subterms t'"
+    apply(rule types_pset_atom.cases[OF \<open>v \<turnstile> a\<close>])
+    using atom(2) by auto
+  then have "\<not> Option.is_none (type_term v t1) \<and> type_term v t1 = type_term v t2"
+  by (induction t' arbitrary: l)
+     (use assms(3) in \<open>(auto simp: type_term.simps split: if_splits Option.bind_splits)\<close>)
+  then show "\<not> Option.is_none (type_term v t1)" "type_term v t1 = type_term v t2"
+    by blast+
+qed
+
+lemma types_if_types_Member_and_subterms:
+  fixes \<phi> :: "'a pset_fm"
+  assumes "v \<turnstile> s \<in>\<^sub>s t1 \<or> v \<turnstile> s \<in>\<^sub>s t2" "v \<turnstile> \<phi>"
+  assumes "f t1 t2 \<in> subterms \<phi>" "f \<in> {(\<squnion>\<^sub>s), (\<sqinter>\<^sub>s), (-\<^sub>s)}"
+  shows "v \<turnstile> s \<in>\<^sub>s f t1 t2"
+proof -
+  from type_term_eq_if_mem_subterms[OF assms(2-)] obtain lt where lt:
+    "type_term v t1 = Some lt" "type_term v t2 = Some lt"
+    by fastforce
+  moreover from assms(1) lt(1,2) obtain ls where
+    "type_term v s = Some ls" "lt = Suc ls"
+    using types_pset_atom.simps by force
+  ultimately show ?thesis
+    using assms
+    by (auto simp: type_term.simps types_pset_atom.simps)
+qed
+  
+lemma types_lexpands:
+  assumes "lexpands b' b" "b \<noteq> []" "\<phi> \<in> set b'"
+  assumes "\<And>(\<phi> :: 'a pset_fm). \<phi> \<in> set b \<Longrightarrow> v \<turnstile> \<phi>"
+  shows "v \<turnstile> \<phi>"
+  using assms
+proof(induction rule: lexpands.induct)
+  case (1 b' b)
+  then show ?case
+    apply(induction rule: lexpands_fm.induct)
+          apply(force dest: types_fmD intro: types_fmI(3))+
+    done
+next
+  case (2 b' b)
+  then show ?case
+  proof(induction rule: lexpands_un.induct)
+    case (1 s t1 t2 b)
+    then show ?thesis
+      apply(auto dest!: types_fmD(5,6) "1"(4) intro!: types_fmI(2,3,4)
+                  intro: types_pset_atom_Member_Union_D)
+      done
+  next
+    case (2 s t1 b t2)
+    then have "v \<turnstile> last b"
+      by auto
+    from types_if_types_Member_and_subterms[OF _ this] 2 show ?case
+      by (auto dest!: "2"(5) types_fmD(6) intro: types_fmI(4))
+  next
+    case (3 s t2 b t1)
+    then have "v \<turnstile> last b"
+      by auto
+    from types_if_types_Member_and_subterms[OF _ this] 3 show ?case
+      by (auto dest!: "3"(5) types_fmD(6) intro: types_fmI(4))
+  next
+    case (4 s t1 t2 b)
+    then show ?case
+      apply(auto dest!: types_fmD(5,6) "4"(5) intro!: types_fmI(2,3,4)
+                 intro: types_pset_atom_Member_Union_D)
+      done
+  next
+    case (5 s t1 t2 b)
+    then show ?case
+      apply(auto dest!: types_fmD(5,6) "5"(5) intro!: types_fmI(2,3,4)
+                 intro: types_pset_atom_Member_Union_D)
+      done
+  next
+    case (6 s t1 b t2)
+    then have "v \<turnstile> last b"
+      by auto
+    note types_if_types_Member_and_subterms[where ?f="(\<squnion>\<^sub>s)", OF _ this "6"(3), simplified]
+    with 6 show ?case
+      apply(auto dest!: types_fmD(5,6) "6"(6) intro!: types_fmI(2,3,4))
+      done
+  qed
+next
+  case (3 b' b)
+  then show ?case
+  proof(induction rule: lexpands_int.induct)
+    case (1 s t1 t2 b)
+    then show ?thesis
+      apply(auto dest!: types_fmD(5,6) "1"(4) intro!: types_fmI(2,3,4)
+                  intro: types_pset_atom_Member_Inter_D)
+      done
+  next
+    case (2 s t1 b t2)
+    then have "v \<turnstile> last b"
+      by auto
+    from types_if_types_Member_and_subterms[OF _ this] 2 show ?case
+      by (auto dest!: "2"(5) types_fmD(5,6) intro!: types_fmI(3,4))
+  next
+    case (3 s t2 b t1)
+    then have "v \<turnstile> last b"
+      by auto
+    from types_if_types_Member_and_subterms[OF _ this] 3 show ?case
+      by (auto dest!: "3"(5) types_fmD(5,6) intro!: types_fmI(3,4))
+  next
+    case (4 s t1 t2 b)
+    then show ?case
+      apply(auto dest!: types_fmD(5,6) "4"(5) intro!: types_fmI(2,3,4)
+                 intro: types_pset_atom_Member_Inter_D)
+      done
+  next
+    case (5 s t1 t2 b)
+    then show ?case
+      apply(auto dest!: types_fmD(5,6) "5"(5) intro!: types_fmI(2,3,4)
+                 intro: types_pset_atom_Member_Inter_D)
+      done
+  next
+    case (6 s t1 b t2)
+    then have "v \<turnstile> last b"
+      by auto
+    note types_if_types_Member_and_subterms[where ?f="(\<sqinter>\<^sub>s)", OF _ this "6"(3), simplified]
+    with 6 show ?case
+      apply(auto dest!: types_fmD(5,6) "6"(6) intro!: types_fmI(2,3,4))
+      done
+  qed
+next
+  case (4 b' b)
+  then show ?case
+    proof(induction rule: lexpands_diff.induct)
+    case (1 s t1 t2 b)
+    then show ?thesis
+      apply(auto dest!: types_fmD(5,6) "1"(4) intro!: types_fmI(2,3,4)
+                  intro: types_pset_atom_Member_Diff_D)
+      done
+  next
+    case (2 s t1 b t2)
+    then have "v \<turnstile> last b"
+      by auto
+    from types_if_types_Member_and_subterms[OF _ this] 2 show ?case
+      by (auto dest!: "2"(5) types_fmD(5,6) intro!: types_fmI(3,4))
+  next
+    case (3 s t2 b t1)
+    then have "v \<turnstile> last b"
+      by auto
+    from types_if_types_Member_and_subterms[OF _ this] 3 show ?case
+      by (auto dest!: "3"(5) types_fmD(5,6) intro!: types_fmI(3,4))
+  next
+    case (4 s t1 t2 b)
+    then show ?case
+      apply(auto dest!: types_fmD(5,6) "4"(5) intro!: types_fmI(2,3,4)
+                 intro: types_pset_atom_Member_Diff_D)
+      done
+  next
+    case (5 s t1 t2 b)
+    then show ?case
+      apply(auto dest!: types_fmD(5,6) "5"(5) intro!: types_fmI(2,3,4)
+                 intro: types_pset_atom_Member_Diff_D)
+      done
+  next
+    case (6 s t1 b t2)
+    then have "v \<turnstile> last b"
+      by auto
+    note types_if_types_Member_and_subterms[where ?f="(-\<^sub>s)", OF _ this "6"(3), simplified]
+    with 6 show ?case
+      apply(auto dest!: types_fmD(5,6) "6"(6) intro!: types_fmI(2,3,4))
+      done
+  qed
+next
+  case (5 b' b)
+  then show ?case
+  proof(induction rule: lexpands_single.induct)
+    case (1 t1 b)
+    then have "v \<turnstile> last b"
+      by auto
+    with \<open>Single t1 \<in> subterms (last b)\<close> obtain a :: "'a pset_atom"
+      where a: "a \<in> atoms (last b)" "Single t1 \<in> subterms a" "v \<turnstile> a"
+      unfolding types_pset_fm_def by (metis UN_E subterms_fm_def)
+    then obtain f s t where
+      "a = f s t" "f \<in> {(=\<^sub>s), (\<in>\<^sub>s)}"
+      by (metis insertCI pset_atom.exhaust)
+    
+    then have "\<not> Option.is_none (type_term v t1)"
+      
+      apply(induction "last b")
+      apply(auto simp: type_term.simps split: if_splits Option.bind_splits) 
+    then show ?case  sorry
+  next
+    case (2 s t1 b)
+    then show ?case sorry
+  next
+    case (3 s t1 b)
+    then show ?case sorry
+  qed
+next
+  case (6 b' b)
+  then show ?case sorry
+qed
+
+end
